wip on LLLM

raft/proof/LeaderLogsLogMatchingProof.v
@@ -3,6 +3,7 @@ Import ListNotations.
 Require Import Omega.
 
 Require Import VerdiTactics.
+Require Import Util.
 Require Import Net.
 Require Import Raft.
 Require Import RaftRefinementInterface.
@@ -21,6 +22,7 @@ Require Import LeaderLogsSortedInterface.
 Require Import SortedInterface.
 Require Import LeaderLogsSublogInterface.
 Require Import AllEntriesLeaderLogsInterface.
+Require Import LeaderLogsContiguousInterface.
 
 Require Import LeaderLogsLogMatchingInterface.
 
@@ -37,11 +39,37 @@ Section LeaderLogsLogMatching.
   Context {si : sorted_interface}.
   Context {aelli : all_entries_leader_logs_interface}.
   Context {llsli : leaderLogs_sublog_interface}.
+  Context {llci : leaderLogs_contiguous_interface}.
+
+  Definition leaderLogs_entries_match_nw (net : network) : Prop :=
+    forall h llt ll p t src pli plt es ci,
+      In (llt, ll) (leaderLogs (fst (nwState net h))) ->
+      In p (nwPackets net) ->
+      pBody p = AppendEntries t src pli plt es ci ->
+      (forall e1 e2,
+         eIndex e1 = eIndex e2 ->
+         eTerm e1 = eTerm e2 ->
+         In e1 es ->
+         In e2 ll ->
+         (forall e3,
+            eIndex e3 <= eIndex e1 ->
+            In e3 es ->
+            In e3 ll) /\
+         (pli <> 0 ->
+          exists e4,
+            eIndex e4 = pli /\
+            eTerm e4 = plt /\
+            In e4 ll)).
+
+  Definition leaderLogs_entries_match (net : network) : Prop :=
+    leaderLogs_entries_match_host net /\
+    leaderLogs_entries_match_nw net.
 
   Lemma leaderLogs_entries_match_init :
-    refined_raft_net_invariant_init leaderLogs_entries_match_host.
+    refined_raft_net_invariant_init leaderLogs_entries_match.
   Proof.
-    unfold refined_raft_net_invariant_init, leaderLogs_entries_match_host.
+    unfold refined_raft_net_invariant_init, leaderLogs_entries_match,
+           leaderLogs_entries_match_host, leaderLogs_entries_match_nw.
     simpl.
     intuition.
   Qed.
@@ -53,7 +81,6 @@ Section LeaderLogsLogMatching.
       | [ |- context [ update _ ?x _ ?y ] ] =>
         destruct (name_eq_dec x y); subst; rewrite_update; simpl in *
     end.
-
 
   Lemma update_elections_data_client_request_leaderLogs :
     forall h st client id c,
@@ -120,8 +147,26 @@ Section LeaderLogsLogMatching.
     intuition.
   Qed.
 
-  Lemma lifted_logs_sorted :
-    forall net h,
+  Lemma lifted_logs_sorted_nw :
+    forall net p t n plt plti es ci,
+      refined_raft_intermediate_reachable net ->
+      In p (nwPackets net) ->
+      pBody p = AppendEntries t n plt plti es ci ->
+      sorted es.
+  Proof.
+    intros.
+    pose proof (lift_prop _ logs_sorted_invariant).
+    find_insterU. conclude_using eauto.
+    unfold logs_sorted in *. break_and.
+    unfold logs_sorted_nw in *.
+    eapply H3.
+    - unfold deghost. simpl.
+      apply in_map_iff. eauto.
+    - simpl. eauto.
+  Qed.
+
+  Lemma lifted_logs_sorted_host :
+    forall net h ,
       refined_raft_intermediate_reachable net ->
       sorted (log (snd (nwState net h))).
   Proof.
@@ -135,81 +180,185 @@ Section LeaderLogsLogMatching.
     eauto.
   Qed.
 
-  Lemma leaderLogs_entries_match_client_request :
-    refined_raft_net_invariant_client_request leaderLogs_entries_match_host.
+  Lemma leaderLogs_entries_match_nw_packet_set :
+    forall net net',
+      (forall p, In p (nwPackets net') ->
+                 is_append_entries (pBody p) ->
+                 In p (nwPackets net)) ->
+      (forall h, leaderLogs (fst (nwState net' h)) = leaderLogs (fst (nwState net h))) ->
+      leaderLogs_entries_match_nw net ->
+      leaderLogs_entries_match_nw net'.
   Proof.
-    unfold refined_raft_net_invariant_client_request, leaderLogs_entries_match_host.
-    simpl. intuition. subst. find_higher_order_rewrite.
-    repeat update_destruct.
-    - rewrite update_elections_data_client_request_leaderLogs in *.
-      destruct (log d) using (handleClientRequest_log_ind $(eauto)$).
-      + eauto.
-      + destruct ll.
-        * apply entries_match_nil.
-        * { apply entries_match_cons_gt_maxTerm; eauto.
-            - eauto using lifted_logs_sorted.
-            - eapply leaderLogs_sorted_invariant; eauto.
-            - omega.
-            - find_copy_apply_lem_hyp leaderLogs_currentTerm_invariant; auto.
-              find_copy_apply_lem_hyp leaderLogs_term_sanity_invariant.
-              unfold leaderLogs_term_sanity in *.
-              eapply_prop_hyp In In; simpl; eauto. repeat find_rewrite.
-              simpl in *. omega.
-          }
-    - rewrite update_elections_data_client_request_leaderLogs in *.
-      eauto.
-    - destruct (log d) using (handleClientRequest_log_ind $(eauto)$).
-      + eauto.
-      + apply entries_match_cons_sublog; eauto.
-        * eauto using lifted_logs_sorted.
-        * eapply leaderLogs_sorted_invariant; eauto.
-        * omega.
-        * intros.
-          eapply leaderLogs_sublog_invariant; eauto.
-          simpl in *. congruence.
-    - eauto.
+    unfold leaderLogs_entries_match_nw.
+    intros.
+    eapply_prop_hyp In nwPackets; [|eauto 10].
+    eapply H1; eauto.
+    repeat find_higher_order_rewrite.
+    eauto.
+  Qed.
+
+  Lemma handleClientRequest_no_send :
+    forall h st client id c out st' ms,
+      handleClientRequest h st client id c = (out, st', ms) ->
+      ms = [].
+  Proof.
+    unfold handleClientRequest.
+    intros.
+    repeat break_match; repeat find_inversion; auto.
+  Qed.
+
+  Lemma leaderLogs_entries_match_client_request :
+    refined_raft_net_invariant_client_request leaderLogs_entries_match.
+  Proof.
+    unfold refined_raft_net_invariant_client_request, leaderLogs_entries_match.
+    intros.
+    split.
+    - { unfold leaderLogs_entries_match_host.
+        simpl. intuition. subst. find_higher_order_rewrite.
+        repeat update_destruct.
+        - rewrite update_elections_data_client_request_leaderLogs in *.
+          destruct (log d) using (handleClientRequest_log_ind $(eauto)$).
+          + eauto.
+          + destruct ll.
+            * apply entries_match_nil.
+            * { apply entries_match_cons_gt_maxTerm; eauto.
+                - eauto using lifted_logs_sorted_host.
+                - eapply leaderLogs_sorted_invariant; eauto.
+                - omega.
+                - find_copy_apply_lem_hyp leaderLogs_currentTerm_invariant; auto.
+                  find_copy_apply_lem_hyp leaderLogs_term_sanity_invariant.
+                  unfold leaderLogs_term_sanity in *.
+                  eapply_prop_hyp In In; simpl; eauto. repeat find_rewrite.
+                  simpl in *. omega.
+              }
+        - rewrite update_elections_data_client_request_leaderLogs in *.
+          eauto.
+        - destruct (log d) using (handleClientRequest_log_ind $(eauto)$).
+          + eauto.
+          + apply entries_match_cons_sublog; eauto.
+            * eauto using lifted_logs_sorted_host.
+            * eapply leaderLogs_sorted_invariant; eauto.
+            * omega.
+            * intros.
+              eapply leaderLogs_sublog_invariant; eauto.
+              simpl in *. congruence.
+        - eauto.
+      }
+    - eapply leaderLogs_entries_match_nw_packet_set with (net:=net); intuition.
+      + find_apply_hyp_hyp. intuition eauto.
+        erewrite handleClientRequest_no_send with (ms := l) in * by eauto.
+        simpl in *. intuition.
+      + simpl. subst. find_higher_order_rewrite.
+        rewrite update_fun_comm. simpl.
+        rewrite update_fun_comm. simpl.
+        rewrite update_elections_data_client_request_leaderLogs.
+        now rewrite update_nop_ext' by auto.
+  Qed.
+
+  Lemma update_elections_data_timeout_leaderLogs :
+    forall h st,
+      leaderLogs (update_elections_data_timeout h st) = leaderLogs (fst st).
+  Proof.
+    unfold update_elections_data_timeout.
+    intros.
+    repeat break_match; auto.
   Qed.
 
   Lemma leaderLogs_entries_match_timeout :
-    refined_raft_net_invariant_timeout leaderLogs_entries_match_host.
-  Admitted.
+    refined_raft_net_invariant_timeout leaderLogs_entries_match.
+  Proof.
+    unfold refined_raft_net_invariant_timeout, leaderLogs_entries_match.
+    intuition.
+    - unfold leaderLogs_entries_match_host in *.
+      intros. simpl in *. repeat find_higher_order_rewrite.
+      repeat update_destruct; rewrite_update;
+      try rewrite update_elections_data_timeout_leaderLogs in *;
+      try erewrite handleTimeout_log_same by eauto; eauto.
+    - eapply leaderLogs_entries_match_nw_packet_set with (net:=net); intuition.
+      + simpl in *. find_apply_hyp_hyp.  intuition.
+        do_in_map. subst. simpl in *.
+        exfalso. eapply handleTimeout_not_is_append_entries; eauto 10.
+      + simpl. repeat find_higher_order_rewrite.
+        rewrite update_fun_comm. simpl.
+        rewrite update_fun_comm. simpl.
+        rewrite update_elections_data_timeout_leaderLogs.
+        rewrite update_nop_ext'; auto.
+  Qed.
+
+  Lemma update_elections_data_appendEntries_leaderLogs :
+    forall h st t src pli plt es ci,
+      leaderLogs (update_elections_data_appendEntries h st t src pli plt es ci) = leaderLogs (fst st).
+  Proof.
+    unfold update_elections_data_appendEntries.
+    intros. repeat break_match; auto.
+  Qed.
 
   Lemma leaderLogs_entries_match_append_entries :
-    refined_raft_net_invariant_append_entries leaderLogs_entries_match_host.
-  Admitted.
+    refined_raft_net_invariant_append_entries leaderLogs_entries_match.
+  Proof.
+    unfold refined_raft_net_invariant_append_entries, leaderLogs_entries_match.
+    intuition.
+    - unfold leaderLogs_entries_match_host in *. intros.
+      {
+        intros. simpl in *. repeat find_higher_order_rewrite.
+        find_rewrite_lem update_fun_comm. simpl in *.
+        find_rewrite_lem update_fun_comm.
+        rewrite update_elections_data_appendEntries_leaderLogs in *.
+        find_erewrite_lem update_nop_ext'.
+        update_destruct; rewrite_update;
+        try rewrite update_elections_data_appendEntries_leaderLogs in *; eauto.
+        destruct (log d) using (handleAppendEntries_log_ind $(eauto)$); eauto.
+        + eapply entries_match_scratch with (plt0 := plt).
+          * eauto using lifted_logs_sorted_nw.
+          * apply sorted_uniqueIndices.
+            eapply leaderLogs_sorted_invariant; eauto.
+          * subst. eapply_prop leaderLogs_entries_match_nw; eauto.
+          * admit.
+          * admit.
+          * admit.
+        + eapply entries_match_append; eauto.
+          * admit.
+          * admit.
+          * admit.
+          * admit.
+          * admit.
+          * eapply findAtIndex_intro; eauto using lifted_logs_sorted_host, sorted_uniqueIndices.
+      }
+    - (* nw *) admit.
+  Qed.
 
   Lemma leaderLogs_entries_match_append_entries_reply :
-    refined_raft_net_invariant_append_entries_reply leaderLogs_entries_match_host.
+    refined_raft_net_invariant_append_entries_reply leaderLogs_entries_match.
   Admitted.
 
   Lemma leaderLogs_entries_match_request_vote :
-    refined_raft_net_invariant_request_vote leaderLogs_entries_match_host.
+    refined_raft_net_invariant_request_vote leaderLogs_entries_match.
   Admitted.
 
   Lemma leaderLogs_entries_match_request_vote_reply :
-    refined_raft_net_invariant_request_vote_reply leaderLogs_entries_match_host.
+    refined_raft_net_invariant_request_vote_reply leaderLogs_entries_match.
   Admitted.
 
   Lemma leaderLogs_entries_match_do_leader :
-    refined_raft_net_invariant_do_leader leaderLogs_entries_match_host.
+    refined_raft_net_invariant_do_leader leaderLogs_entries_match.
   Admitted.
 
   Lemma leaderLogs_entries_match_do_generic_server :
-    refined_raft_net_invariant_do_generic_server leaderLogs_entries_match_host.
+    refined_raft_net_invariant_do_generic_server leaderLogs_entries_match.
   Admitted.
 
   Lemma leaderLogs_entries_match_state_same_packet_subset :
-    refined_raft_net_invariant_state_same_packet_subset leaderLogs_entries_match_host.
+    refined_raft_net_invariant_state_same_packet_subset leaderLogs_entries_match.
   Admitted.
 
   Lemma leaderLogs_entries_match_reboot :
-    refined_raft_net_invariant_reboot leaderLogs_entries_match_host.
+    refined_raft_net_invariant_reboot leaderLogs_entries_match.
   Admitted.
 
   Lemma leaderLogs_entries_match_invariant :
     forall net,
       refined_raft_intermediate_reachable net ->
-      leaderLogs_entries_match_host net.
+      leaderLogs_entries_match net.
   Proof.
     intros.
     apply refined_raft_net_invariant; auto.
@@ -229,6 +378,6 @@ Section LeaderLogsLogMatching.
   Instance lllmi : leaderLogs_entries_match_interface : Prop.
   Proof.
     split.
-    exact leaderLogs_entries_match_invariant.
+    apply leaderLogs_entries_match_invariant.
   Qed.
 End LeaderLogsLogMatching.
